Pre-cond for merge

inductive_proof/Append-only_log/App.fst
@@ -2,7 +2,6 @@ module App
 
 open FStar.Seq
 open FStar.Ghost
-module L = FStar.List.Tot
 
 #set-options "--query_stats"
 // the concrete state type
@@ -34,8 +33,15 @@ let eq_is_equiv (a b:concrete_st)
 // (the only operation is append, so unit is fine)
 type app_op_t:eqtype = unit
 
+let is_prefix_s (p l:concrete_st) : Tot prop =
+  Seq.length l >= Seq.length p /\ Seq.equal p (Seq.slice l 0 (Seq.length p))
+
+let is_suffix_s (s l:concrete_st) : Tot prop =
+  Seq.length l >= Seq.length s /\ Seq.equal s (Seq.slice l (Seq.length l - Seq.length s) (Seq.length l))
+
 // apply an operation to a state
-let do (s:concrete_st) (op:op_t) : concrete_st = cons (fst op) s
+let do (s:concrete_st) (op:op_t) : concrete_st =
+  cons (fst op) s
 
 let lem_do (a b:concrete_st) (op:op_t)
    : Lemma (requires eq a b)
@@ -53,409 +59,189 @@ let resolve_conflict_prop (x y:op_t)
                    (last (resolve_conflict x y) <> x <==> lt (fst x) (fst y)))
   = ()
 
-#push-options "--z3rlimit 50"
-let rec union_s (l1 l2:concrete_st) : Tot concrete_st
+let rec union_s (l1 l2:concrete_st) 
+  : Tot (u:concrete_st{forall e. mem e u <==> mem e l1 \/ mem e l2}) 
   (decreases %[length l1; length l2]) =
   match length l1, length l2 with
   |0, 0 -> empty
   |0, _ -> l2
   |_, 0 -> l1
-  |_, _ -> if (head l1 >= head l2) 
+  |_, _ ->  if (head l1 >= head l2) 
              then (mem_cons (head l1) (union_s (tail l1) l2);
                    cons (head l1) (union_s (tail l1) l2))
              else (mem_cons (head l2) (union_s l1 (tail l2));
                    cons (head l2) (union_s l1 (tail l2)))
-#pop-options
 
-let is_prefix_s (p l:concrete_st) : Tot prop =
-  Seq.length l >= Seq.length p /\ Seq.equal p (Seq.slice l 0 (Seq.length p))
-
-let is_suffix_s (s l:concrete_st) : Tot prop =
-  Seq.length l >= Seq.length s /\ Seq.equal s (Seq.slice l (Seq.length l - Seq.length s) (Seq.length l))
-  
 let diff_s (s1:concrete_st) (lca:concrete_st{is_suffix_s lca s1}) 
   : Tot (d:concrete_st{s1 == Seq.append d lca}) =
   let s = fst (split s1 (length s1 - length lca)) in
   lemma_split s1 (length s1 - length lca);
   lemma_mem_append s lca;
   s
-  
-// concrete merge pre
-let concrete_merge_pre (lca s1 s2:concrete_st) = 
-  is_suffix_s lca s1 /\
-  is_suffix_s lca s2
 
-#push-options "--z3rlimit 50"
-let concrete_merge (lca s1:concrete_st) (s2:concrete_st{concrete_merge_pre lca s1 s2}) : concrete_st =
+let rec lem_foldl (s:concrete_st) (l:log)
+  : Lemma (requires true)
+          (ensures (length l = 0 ==> (apply_log s l = s)) /\
+                   (is_suffix_s s (apply_log s l)))
+          (decreases length l)
+          [SMTPat (is_suffix_s s (apply_log s l))]
+  = match length l with
+    |0 -> ()
+    |1 -> ()
+    |_ -> assert (is_suffix_s s (do s (head l)));
+         lem_foldl (do s (head l)) (tail l)
+
+let lem_foldl_forall (s:concrete_st) 
+  : Lemma (ensures (forall l. (is_suffix_s s (apply_log s l)))) = ()
+
+let concrete_merge (lca s1 s2:concrete_st) 
+  : Pure concrete_st
+         (requires (exists l1 l2. apply_log lca l1 == s1 /\ apply_log lca l2 == s2))
+         (ensures (fun _ -> True)) = 
+  //lem_foldl_forall lca;
   let la = diff_s s1 lca in
   let lb = diff_s s2 lca in
   let u = union_s la lb in 
   lemma_mem_append u lca;
   Seq.append u lca
 
-let linearizable_s1_0''_base_pre (lca s1 s2':st) (last2:op_t)
-  : Lemma (requires is_prefix (ops_of lca) (ops_of s1) /\
-                    is_prefix (ops_of lca) (ops_of s2') /\
-                    is_prefix (ops_of lca) (snoc (ops_of s2') last2) /\
-                    ops_of s1 == ops_of lca /\ ops_of s2' == ops_of lca /\
-                    (forall id id1. mem_id id (ops_of lca) /\ mem_id id1 (diff (ops_of s1) (ops_of lca)) ==> lt id id1) /\
-                    (forall id id1. mem_id id (ops_of lca) /\ mem_id id1 (diff (ops_of s2') (ops_of lca)) ==> lt id id1) /\
-                    (forall id. mem_id id (diff (ops_of s1) (ops_of lca)) ==> not (mem_id id (diff (ops_of s2') (ops_of lca)))) /\
-                    (forall id. mem_id id (ops_of lca) ==> lt id (fst last2)) /\
-                    concrete_merge_pre (v_of lca) (v_of s1) (do (v_of s2') last2) /\
-                    length (ops_of lca) > 0)
-        
-          (ensures (let l' = inverse_st lca in
-                    let s1' = inverse_st s1 in
-                    let s2'' = inverse_st s2' in
-                    concrete_merge_pre (v_of l') (v_of s1') (do (v_of s2'') last2))) = ()
-
 let linearizable_s1_0''_base_base (lca s1 s2':st) (last2:op_t)
-  : Lemma (requires is_prefix (ops_of lca) (ops_of s1) /\
-                    is_prefix (ops_of lca) (ops_of s2') /\
+  : Lemma (requires consistent_branches lca s1 s2' /\
                     is_prefix (ops_of lca) (snoc (ops_of s2') last2) /\
-                    ops_of s1 == ops_of lca /\ ops_of s2' == ops_of lca /\
+                    ops_of s1 = ops_of lca /\ ops_of s2' = ops_of lca /\
                     length (ops_of lca) = 0 /\
-                    (forall id id1. mem_id id (ops_of lca) /\ mem_id id1 (diff (ops_of s1) (ops_of lca)) ==> lt id id1) /\
-                    (forall id id1. mem_id id (ops_of lca) /\ mem_id id1 (diff (ops_of s2') (ops_of lca)) ==> lt id id1) /\
-                    (forall id. mem_id id (diff (ops_of s1) (ops_of lca)) ==> not (mem_id id (diff (ops_of s2') (ops_of lca)))) /\
-                    (forall id. mem_id id (ops_of lca) ==> lt id (fst last2)) /\
-                    concrete_merge_pre (v_of lca) (v_of s1) (do (v_of s2') last2))
+                    (forall id. mem_id id (ops_of lca) ==> lt id (fst last2)))
         
           (ensures eq (do (v_of s2') last2) (concrete_merge (v_of lca) (v_of s1) (do (v_of s2') last2))) = ()
 
-let linearizable_s1_0''_pre (lca s1 s2':st) (last2:op_t)
-  : Lemma (requires is_prefix (ops_of lca) (ops_of s1) /\
-                    is_prefix (ops_of lca) (ops_of s2') /\
-                    is_prefix (ops_of lca) (snoc (ops_of s2') last2) /\
-                    ops_of s1 == ops_of lca /\
-                    (forall id id1. mem_id id (ops_of lca) /\ mem_id id1 (diff (ops_of s1) (ops_of lca)) ==> lt id id1) /\
-                    (forall id id1. mem_id id (ops_of lca) /\ mem_id id1 (diff (ops_of s2') (ops_of lca)) ==> lt id id1) /\
-                    (forall id. mem_id id (diff (ops_of s1) (ops_of lca)) ==> not (mem_id id (diff (ops_of s2') (ops_of lca)))) /\
-                    (forall id. mem_id id (ops_of lca) ==> lt id (fst last2)) /\
-                    concrete_merge_pre (v_of lca) (v_of s1) (do (v_of s2') last2) /\
-                    length (ops_of s2') > length (ops_of lca))
-         
-          (ensures (let inv2 = inverse_st s2' in
-                    concrete_merge_pre (v_of lca) (v_of s1) (do (v_of inv2) last2))) = admit()
-
+#push-options "--z3rlimit 50"
 let linearizable_s1_0''_base_ind (lca s1 s2':st) (last2:op_t)
-  : Lemma (requires is_prefix (ops_of lca) (ops_of s1) /\
-                    is_prefix (ops_of lca) (ops_of s2') /\
+  : Lemma (requires consistent_branches lca s1 s2' /\
                     is_prefix (ops_of lca) (snoc (ops_of s2') last2) /\
-                    ops_of s1 == ops_of lca /\ ops_of s2' == ops_of lca /\
+                    ops_of s1 = ops_of lca /\ ops_of s2' = ops_of lca /\
                     length (ops_of lca) > 0 /\
-                    (forall id id1. mem_id id (ops_of lca) /\ mem_id id1 (diff (ops_of s1) (ops_of lca)) ==> lt id id1) /\
-                    (forall id id1. mem_id id (ops_of lca) /\ mem_id id1 (diff (ops_of s2') (ops_of lca)) ==> lt id id1) /\
-                    (forall id. mem_id id (diff (ops_of s1) (ops_of lca)) ==> not (mem_id id (diff (ops_of s2') (ops_of lca)))) /\
                     (forall id. mem_id id (ops_of lca) ==> lt id (fst last2)) /\
 
                     (let l' = inverse_st lca in
                     let s1' = inverse_st s1 in
                     let s2'' = inverse_st s2' in
-                    is_prefix (ops_of l') (ops_of s1') /\ 
-                    is_prefix (ops_of l') (ops_of s2'') /\
+                    consistent_branches l' s1' s2'' /\
                     is_prefix (ops_of l') (snoc (ops_of s2'') last2) /\
                     ops_of s1' = ops_of l' /\ ops_of s2'' = ops_of l' /\
-                    (forall id id1. mem_id id (ops_of l') /\ mem_id id1 (diff (ops_of s1') (ops_of l')) ==> lt id id1) /\
-                    (forall id id1. mem_id id (ops_of l') /\ mem_id id1 (diff (ops_of s2'') (ops_of l')) ==> lt id id1) /\
-                    (forall id. mem_id id (diff (ops_of s1') (ops_of l')) ==> not (mem_id id (diff (ops_of s2'') (ops_of l')))) /\
-                    concrete_merge_pre (v_of lca) (v_of s1) (do (v_of s2') last2) /\
-                    concrete_merge_pre (v_of l') (v_of s1') (do (v_of s2'') last2) /\
                     eq (do (v_of s2'') last2) (concrete_merge (v_of l') (v_of s1') (do (v_of s2'') last2))))
 
           (ensures eq (do (v_of s2') last2) (concrete_merge (v_of lca) (v_of s1) (do (v_of s2') last2))) = ()
-          
+#pop-options
+
 let linearizable_s1_0''_ind (lca s1 s2':st) (last2:op_t)
-  : Lemma (requires is_prefix (ops_of lca) (ops_of s1) /\
-                    is_prefix (ops_of lca) (ops_of s2') /\
+  : Lemma (requires consistent_branches_s2_gt0 lca s1 s2' /\
                     is_prefix (ops_of lca) (snoc (ops_of s2') last2) /\
-                    ops_of s1 == ops_of lca /\
-                    length (ops_of s2') > length (ops_of lca) /\
-                    (forall id id1. mem_id id (ops_of lca) /\ mem_id id1 (diff (ops_of s1) (ops_of lca)) ==> lt id id1) /\
-                    (forall id id1. mem_id id (ops_of lca) /\ mem_id id1 (diff (ops_of s2') (ops_of lca)) ==> lt id id1) /\
-                    (forall id. mem_id id (diff (ops_of s1) (ops_of lca)) ==> not (mem_id id (diff (ops_of s2') (ops_of lca)))) /\
+                    ops_of s1 = ops_of lca /\
                     (forall id. mem_id id (ops_of lca) ==> lt id (fst last2)) /\
 
                     (let inv2 = inverse_st s2' in
-                    is_prefix (ops_of lca) (ops_of inv2) /\
+                    consistent_branches lca s1 inv2 /\
                     is_prefix (ops_of lca) (snoc (ops_of inv2) last2) /\
-                    (forall id id1. mem_id id (ops_of lca) /\ mem_id id1 (diff (ops_of inv2) (ops_of lca)) ==> lt id id1) /\
-                    (forall id. mem_id id (diff (ops_of s1) (ops_of lca)) ==> not (mem_id id (diff (ops_of inv2) (ops_of lca)))) /\
-                    concrete_merge_pre (v_of lca) (v_of s1) (do (v_of s2') last2) /\
-                    concrete_merge_pre (v_of lca) (v_of s1) (do (v_of inv2) last2) /\
+                    (exists l2. do (v_of inv2) last2 == apply_log (v_of lca) l2) /\
+                    (exists l2. do (v_of s2') last2 == apply_log (v_of lca) l2) /\                    
                     eq (do (v_of inv2) last2) (concrete_merge (v_of lca) (v_of s1) (do (v_of inv2) last2))))
         
           (ensures eq (do (v_of s2') last2) (concrete_merge (v_of lca) (v_of s1) (do (v_of s2') last2))) = ()
-          
+
 let linearizable_s1_0_s2_0_base (lca s1 s2:st)
-  : Lemma (requires is_prefix (ops_of lca) (ops_of s1) /\
-                    is_prefix (ops_of lca) (ops_of s2) /\
-                    ops_of s1 == ops_of lca /\ ops_of s2 == ops_of lca /\
-                    (forall id id1. mem_id id (ops_of lca) /\ mem_id id1 (diff (ops_of s1) (ops_of lca)) ==> lt id id1) /\
-                    (forall id id1. mem_id id (ops_of lca) /\ mem_id id1 (diff (ops_of s2) (ops_of lca)) ==> lt id id1) /\
-                    (forall id. mem_id id (diff (ops_of s1) (ops_of lca)) ==> not (mem_id id (diff (ops_of s2) (ops_of lca)))) /\
-                    concrete_merge_pre (v_of lca) (v_of s1) (v_of s2))
+  : Lemma (requires consistent_branches lca s1 s2 /\
+                    ops_of s1 = ops_of lca /\ ops_of s2 = ops_of lca /\
+                    (exists l2. (v_of s2) == apply_log (v_of lca) l2) /\
+                    (exists l1. (v_of s1) == apply_log (v_of lca) l1))
         
           (ensures eq (v_of lca) (concrete_merge (v_of lca) (v_of s1) (v_of s2))) = ()
 
-let linearizable_s2_0''_base_pre (lca s1' s2:st) (last1:op_t)
-  : Lemma (requires is_prefix (ops_of lca) (ops_of s1') /\
-                    is_prefix (ops_of lca) (ops_of s2) /\
-                    is_prefix (ops_of lca) (snoc (ops_of s1') last1) /\
-                    ops_of s1' == ops_of lca /\ ops_of s2 == ops_of lca /\
-                    (forall id id1. mem_id id (ops_of lca) /\ mem_id id1 (diff (ops_of s1') (ops_of lca)) ==> lt id id1) /\
-                    (forall id id1. mem_id id (ops_of lca) /\ mem_id id1 (diff (ops_of s2) (ops_of lca)) ==> lt id id1) /\
-                    (forall id. mem_id id (diff (ops_of s1') (ops_of lca)) ==> not (mem_id id (diff (ops_of s2) (ops_of lca)))) /\
-                    (forall id. mem_id id (ops_of lca) ==> lt id (fst last1)) /\
-                    concrete_merge_pre (v_of lca) (do (v_of s1') last1) (v_of s2) /\
-                    length (ops_of lca) > 0)
-         
-          (ensures (let l' = inverse_st lca in
-                    let s1'' = inverse_st s1' in
-                    let s2' = inverse_st s2 in
-                    concrete_merge_pre (v_of l') (do (v_of s1'') last1) (v_of s2'))) = ()
-
 let linearizable_s2_0''_base_base (lca s1' s2:st) (last1:op_t)
-  : Lemma (requires is_prefix (ops_of lca) (ops_of s1') /\
-                    is_prefix (ops_of lca) (ops_of s2) /\
+  : Lemma (requires consistent_branches lca s1' s2 /\
                     is_prefix (ops_of lca) (snoc (ops_of s1') last1) /\
-                    ops_of s1' == ops_of lca /\ ops_of s2 == ops_of lca /\
+                    ops_of s1' = ops_of lca /\ ops_of s2 = ops_of lca /\
                     length (ops_of lca) = 0 /\
-                    (forall id id1. mem_id id (ops_of lca) /\ mem_id id1 (diff (ops_of s1') (ops_of lca)) ==> lt id id1) /\
-                    (forall id id1. mem_id id (ops_of lca) /\ mem_id id1 (diff (ops_of s2) (ops_of lca)) ==> lt id id1) /\
-                    (forall id. mem_id id (diff (ops_of s1') (ops_of lca)) ==> not (mem_id id (diff (ops_of s2) (ops_of lca)))) /\
-                    (forall id. mem_id id (ops_of lca) ==> lt id (fst last1)) /\
-                    concrete_merge_pre (v_of lca) (do (v_of s1') last1) (v_of s2))
+                    (forall id. mem_id id (ops_of lca) ==> lt id (fst last1)))
          
           (ensures eq (do (v_of s1') last1) (concrete_merge (v_of lca) (do (v_of s1') last1) (v_of s2))) = ()
 
-let linearizable_s2_0''_pre (lca s1' s2:st) (last1:op_t)
-  : Lemma (requires is_prefix (ops_of lca) (ops_of s1') /\
-                    is_prefix (ops_of lca) (ops_of s2) /\
-                    is_prefix (ops_of lca) (snoc (ops_of s1') last1) /\
-                    ops_of s2 == ops_of lca /\
-                    (forall id id1. mem_id id (ops_of lca) /\ mem_id id1 (diff (ops_of s1') (ops_of lca)) ==> lt id id1) /\
-                    (forall id id1. mem_id id (ops_of lca) /\ mem_id id1 (diff (ops_of s2) (ops_of lca)) ==> lt id id1) /\
-                    (forall id. mem_id id (diff (ops_of s1') (ops_of lca)) ==> not (mem_id id (diff (ops_of s2) (ops_of lca)))) /\
-                    (forall id. mem_id id (ops_of lca) ==> lt id (fst last1)) /\
-                    concrete_merge_pre (v_of lca) (do (v_of s1') last1) (v_of s2) /\
-                    length (ops_of s1') > length (ops_of lca))
-         
-          (ensures (let inv1 = inverse_st s1' in
-                    concrete_merge_pre (v_of lca) (do (v_of inv1) last1) (v_of s2))) = admit()
-
+#push-options "--z3rlimit 50"
 let linearizable_s2_0''_base_ind (lca s1' s2:st) (last1:op_t)
-  : Lemma (requires is_prefix (ops_of lca) (ops_of s1') /\
-                    is_prefix (ops_of lca) (ops_of s2) /\
+  : Lemma (requires consistent_branches lca s1' s2 /\
                     is_prefix (ops_of lca) (snoc (ops_of s1') last1) /\
-                    ops_of s1' == ops_of lca /\ ops_of s2 == ops_of lca /\
+                    ops_of s1' = ops_of lca /\ ops_of s2 = ops_of lca /\
                     length (ops_of lca) > 0 /\
-                    (forall id id1. mem_id id (ops_of lca) /\ mem_id id1 (diff (ops_of s1') (ops_of lca)) ==> lt id id1) /\
-                    (forall id id1. mem_id id (ops_of lca) /\ mem_id id1 (diff (ops_of s2) (ops_of lca)) ==> lt id id1) /\
-                    (forall id. mem_id id (diff (ops_of s1') (ops_of lca)) ==> not (mem_id id (diff (ops_of s2) (ops_of lca)))) /\
                     (forall id. mem_id id (ops_of lca) ==> lt id (fst last1)) /\
 
                     (let l' = inverse_st lca in
                     let s1'' = inverse_st s1' in
                     let s2' = inverse_st s2 in
-                    is_prefix (ops_of l') (ops_of s1'') /\ 
-                    is_prefix (ops_of l') (ops_of s2') /\
+                    consistent_branches l' s1'' s2' /\
                     is_prefix (ops_of l') (snoc (ops_of s1'') last1) /\
                     ops_of s1'' = ops_of l' /\ ops_of s2' = ops_of l' /\
-                    (forall id id1. mem_id id (ops_of l') /\ mem_id id1 (diff (ops_of s1'') (ops_of l')) ==> lt id id1) /\
-                    (forall id id1. mem_id id (ops_of l') /\ mem_id id1 (diff (ops_of s2') (ops_of l')) ==> lt id id1) /\
-                    (forall id. mem_id id (diff (ops_of s1'') (ops_of l')) ==> not (mem_id id (diff (ops_of s2') (ops_of l')))) /\
-                    concrete_merge_pre (v_of lca) (do (v_of s1') last1) (v_of s2) /\
-                    concrete_merge_pre (v_of l') (do (v_of s1'') last1) (v_of s2') /\
                     eq (do (v_of s1'') last1) (concrete_merge (v_of l') (do (v_of s1'') last1) (v_of s2'))))
 
           (ensures eq (do (v_of s1') last1) (concrete_merge (v_of lca) (do (v_of s1') last1) (v_of s2))) = ()
-          
+#pop-options
+
 let linearizable_s2_0''_ind (lca s1' s2:st) (last1:op_t)
-  : Lemma (requires is_prefix (ops_of lca) (ops_of s1') /\
-                    is_prefix (ops_of lca) (ops_of s2) /\
+  : Lemma (requires consistent_branches_s1_gt0 lca s1' s2 /\
                     is_prefix (ops_of lca) (snoc (ops_of s1') last1) /\
-                    ops_of s2 == ops_of lca /\
-                    length (ops_of s1') > length (ops_of lca) /\
-                    (forall id id1. mem_id id (ops_of lca) /\ mem_id id1 (diff (ops_of s1') (ops_of lca)) ==> lt id id1) /\
-                    (forall id id1. mem_id id (ops_of lca) /\ mem_id id1 (diff (ops_of s2) (ops_of lca)) ==> lt id id1) /\
-                    (forall id. mem_id id (diff (ops_of s1') (ops_of lca)) ==> not (mem_id id (diff (ops_of s2) (ops_of lca)))) /\
+                    ops_of s2 = ops_of lca /\
                     (forall id. mem_id id (ops_of lca) ==> lt id (fst last1)) /\
 
                     (let inv1 = inverse_st s1' in
-                    is_prefix (ops_of lca) (ops_of inv1) /\
+                    consistent_branches lca inv1 s2 /\
                     is_prefix (ops_of lca) (snoc (ops_of inv1) last1) /\
-                    (forall id id1. mem_id id (ops_of lca) /\ mem_id id1 (diff (ops_of inv1) (ops_of lca)) ==> lt id id1) /\
-                    (forall id. mem_id id (diff (ops_of inv1) (ops_of lca)) ==> not (mem_id id (diff (ops_of s2) (ops_of lca)))) /\
-                    concrete_merge_pre (v_of lca) (do (v_of s1') last1) (v_of s2) /\
-                    concrete_merge_pre (v_of lca) (do (v_of inv1) last1) (v_of s2) /\
+                    (exists l1. (do (v_of inv1) last1 == apply_log (v_of lca) l1)) /\
+                    (exists l1. (do (v_of s1') last1 == apply_log (v_of lca) l1)) /\
                     eq (do (v_of inv1) last1) (concrete_merge (v_of lca) (do (v_of inv1) last1) (v_of s2))))
          
           (ensures eq (do (v_of s1') last1) (concrete_merge (v_of lca) (do (v_of s1') last1) (v_of s2))) = ()
 
-let linearizable_gt0_s2'_s10_pre (lca s1 s2:st) (last1 last2:op_t)
-  : Lemma (requires is_prefix (ops_of lca) (ops_of s1) /\
-                    is_prefix (ops_of lca) (ops_of s2) /\
-                    ops_of s1 == ops_of lca /\
-                    fst last1 <> fst last2 /\
-                    last (resolve_conflict last1 last2) <> last1 /\
-                    (forall id id1. mem_id id (ops_of lca) /\ mem_id id1 (diff (ops_of s1) (ops_of lca)) ==> lt id id1) /\
-                    (forall id id1. mem_id id (ops_of lca) /\ mem_id id1 (diff (ops_of s2) (ops_of lca)) ==> lt id id1) /\
-                    (forall id. mem_id id (diff (ops_of s1) (ops_of lca)) ==> not (mem_id id (diff (ops_of s2) (ops_of lca)))) /\
-                    concrete_merge_pre (v_of lca) (do (v_of s1) last1) (do (v_of s2) last2) /\
-                    concrete_merge_pre (v_of lca) (do (v_of s1) last1) (v_of s2) /\
-                    length (ops_of s2) > length (ops_of lca))
-         
-          (ensures (let s2' = inverse_st s2 in
-                   concrete_merge_pre (v_of lca) (do (v_of s1) last1) (do (v_of s2') last2) /\
-                   concrete_merge_pre (v_of lca) (do (v_of s1) last1) (v_of s2'))) = admit()
-
-let linearizable_gt0_s2'_pre (lca s1 s2:st) (last1 last2:op_t)
-  : Lemma (requires is_prefix (ops_of lca) (ops_of s1) /\
-                    is_prefix (ops_of lca) (ops_of s2) /\ 
-                    fst last1 <> fst last2 /\
-                    last (resolve_conflict last1 last2) <> last1 /\
-                    (forall id id1. mem_id id (ops_of lca) /\ mem_id id1 (diff (ops_of s1) (ops_of lca)) ==> lt id id1) /\
-                    (forall id id1. mem_id id (ops_of lca) /\ mem_id id1 (diff (ops_of s2) (ops_of lca)) ==> lt id id1) /\
-                    (forall id. mem_id id (diff (ops_of s1) (ops_of lca)) ==> not (mem_id id (diff (ops_of s2) (ops_of lca)))) /\
-                    concrete_merge_pre (v_of lca) (do (v_of s1) last1) (do (v_of s2) last2) /\
-                    concrete_merge_pre (v_of lca) (do (v_of s1) last1) (v_of s2) /\
-                    length (ops_of s1) > length (ops_of lca))
-         
-          (ensures (let s1' = inverse_st s1 in
-                    concrete_merge_pre (v_of lca) (do (v_of s1') last1) (do (v_of s2) last2) /\
-                    concrete_merge_pre (v_of lca) (do (v_of s1') last1) (v_of s2))) = admit()
-
-let linearizable_gt0_s1'_s20_pre (lca s1 s2:st) (last1 last2:op_t)
-  : Lemma (requires is_prefix (ops_of lca) (ops_of s1) /\
-                    is_prefix (ops_of lca) (ops_of s2) /\
-                    ops_of s2 == ops_of lca /\
-                    fst last1 <> fst last2 /\
-                    last (resolve_conflict last1 last2) = last1 /\
-                    (forall id id1. mem_id id (ops_of lca) /\ mem_id id1 (diff (ops_of s1) (ops_of lca)) ==> lt id id1) /\
-                    (forall id id1. mem_id id (ops_of lca) /\ mem_id id1 (diff (ops_of s2) (ops_of lca)) ==> lt id id1) /\
-                    (forall id. mem_id id (diff (ops_of s1) (ops_of lca)) ==> not (mem_id id (diff (ops_of s2) (ops_of lca)))) /\
-                    concrete_merge_pre (v_of lca) (do (v_of s1) last1) (do (v_of s2) last2) /\
-                    concrete_merge_pre (v_of lca) (v_of s1) (do (v_of s2) last2) /\
-                    length (ops_of s1) > length (ops_of lca))
-        
-          (ensures (let s1' = inverse_st s1 in
-                    concrete_merge_pre (v_of lca) (do (v_of s1') last1) (do (v_of s2) last2) /\
-                    concrete_merge_pre (v_of lca) (v_of s1') (do (v_of s2) last2))) = admit()
-
-let linearizable_gt0_s1'_pre (lca s1 s2:st) (last1 last2:op_t)
-  : Lemma (requires is_prefix (ops_of lca) (ops_of s1) /\
-                    is_prefix (ops_of lca) (ops_of s2) /\
-                    fst last1 <> fst last2 /\
-                    last (resolve_conflict last1 last2) = last1 /\
-                    (forall id id1. mem_id id (ops_of lca) /\ mem_id id1 (diff (ops_of s1) (ops_of lca)) ==> lt id id1) /\
-                    (forall id id1. mem_id id (ops_of lca) /\ mem_id id1 (diff (ops_of s2) (ops_of lca)) ==> lt id id1) /\
-                    (forall id. mem_id id (diff (ops_of s1) (ops_of lca)) ==> not (mem_id id (diff (ops_of s2) (ops_of lca)))) /\
-                    concrete_merge_pre (v_of lca) (do (v_of s1) last1) (do (v_of s2) last2) /\
-                    concrete_merge_pre (v_of lca) (v_of s1) (do (v_of s2) last2) /\
-                    length (ops_of s2) > length (ops_of lca))
-       
-          (ensures (let s2' = inverse_st s2 in
-                    concrete_merge_pre (v_of lca) (do (v_of s1) last1) (do (v_of s2') last2) /\
-                    concrete_merge_pre (v_of lca) (v_of s1) (do (v_of s2') last2))) = admit()
-
-let union_single (a b:concrete_st) (op1 op2:nat)
-  : Lemma (requires a == cons op1 empty /\
-                    b == cons op2 empty /\
-                    op1 > op2)
-          (ensures union_s a b == cons op1 (cons op2 empty)) = ()
-
-let lem_app (op1 op2:nat) (a:concrete_st)
-  : Lemma (ensures Seq.append (cons op1 (cons op2 empty)) a ==
-                   (cons op1 (cons op2 a))) = admit()
-                   
+#push-options "--z3rlimit 50"
 let linearizable_gt0_base_last1 (lca s1 s2:st) (last1 last2:op_t)
-  : Lemma (requires is_prefix (ops_of lca) (ops_of s1) /\
-                    is_prefix (ops_of lca) (ops_of s2) /\
-                    ops_of s1 == ops_of lca /\ ops_of s2 == ops_of lca /\
+  : Lemma (requires consistent_branches lca s1 s2 /\
+                    ops_of s1 = ops_of lca /\ ops_of s2 = ops_of lca /\
                     fst last1 <> fst last2 /\ 
-                    concrete_merge_pre (v_of lca) (do (v_of s1) last1) (do (v_of s2) last2) /\
-                    last (resolve_conflict last1 last2) = last1 /\
-                    concrete_merge_pre (v_of lca) (v_of s1) (do (v_of s2) last2) /\
-                      
-                    (forall id id1. mem_id id (ops_of lca) /\ mem_id id1 (diff (ops_of s1) (ops_of lca)) ==> lt id id1) /\
-                    (forall id id1. mem_id id (ops_of lca) /\ mem_id id1 (diff (ops_of s2) (ops_of lca)) ==> lt id id1) /\
-                    (forall id. mem_id id (diff (ops_of s1) (ops_of lca)) ==> not (mem_id id (diff (ops_of s2) (ops_of lca)))))
+                    (exists l2. (do (v_of s2) last2 == apply_log (v_of lca) l2)) /\
+                    (exists l1. (do (v_of s1) last1 == apply_log (v_of lca) l1)) /\
+                    last (resolve_conflict last1 last2) = last1)
          
           (ensures (eq (do (concrete_merge (v_of lca) (v_of s1) (do (v_of s2) last2)) last1)
-                       (concrete_merge (v_of lca) (do (v_of s1) last1) (do (v_of s2) last2)))) = 
-  assert (fst last1 > fst last2);
-  assert (do (concrete_merge (v_of lca) (v_of s1) (do (v_of s2) last2)) last1 =
-         (cons (fst last1) (cons (fst last2) (v_of lca))));
-  assert ((do (v_of s1) last1) = cons (fst last1) (v_of lca));
-  let s = fst (split (cons (fst last1) (v_of lca)) (length (cons (fst last1) (v_of lca)) - length (v_of lca))) in
-  lemma_split (cons (fst last1) (v_of lca)) (length (cons (fst last1) (v_of lca)) - length (v_of lca));
-  lemma_mem_append s (v_of lca);
-  assert (diff_s (cons (fst last1) (v_of lca)) (v_of lca) == cons (fst last1) empty);
-  assert ((do (v_of s2) last2) = cons (fst last2) (v_of lca));
-  let s = fst (split (cons (fst last2) (v_of lca)) (length (cons (fst last2) (v_of lca)) - length (v_of lca))) in
-  lemma_split (cons (fst last2) (v_of lca)) (length (cons (fst last2) (v_of lca)) - length (v_of lca));
-  lemma_mem_append s (v_of lca);
-  assert (diff_s (cons (fst last2) (v_of lca)) (v_of lca) == cons (fst last2) empty); 
-  union_single (cons (fst last1) empty) (cons (fst last2) empty) (fst last1) (fst last2);
-  let u = union_s (cons (fst last1) empty) (cons (fst last2) empty) in
-  lem_app (fst last1) (fst last2) (v_of lca);
-  assert (Seq.append u (v_of lca) == (cons (fst last1) (cons (fst last2) (v_of lca)))); 
-  assert (concrete_merge (v_of lca) (do (v_of s1) last1) (do (v_of s2) last2) ==
-          (cons (fst last1) (cons (fst last2) (v_of lca)))); ()
+                       (concrete_merge (v_of lca) (do (v_of s1) last1) (do (v_of s2) last2)))) =
+  assert (do (concrete_merge (v_of lca) (v_of s1) (do (v_of s2) last2)) last1 ==
+          cons (fst last1) (cons (fst last2) (v_of lca)));
+  lemma_mem_append (create 1 (fst last2)) (v_of lca);
+  append_assoc (create 1 (fst last1)) (create 1 (fst last2)) (v_of lca);
+  assert (cons (fst last1) (cons (fst last2) (v_of lca)) ==
+          Seq.append (cons (fst last1) (cons (fst last2) empty)) (v_of lca));
+  ()
 
 let linearizable_gt0_base_last2 (lca s1 s2:st) (last1 last2:op_t)
-  : Lemma (requires is_prefix (ops_of lca) (ops_of s1) /\
-                    is_prefix (ops_of lca) (ops_of s2) /\
-                    ops_of s1 == ops_of lca /\ ops_of s2 == ops_of lca /\
+  : Lemma (requires consistent_branches lca s1 s2 /\
+                    ops_of s1 = ops_of lca /\ ops_of s2 = ops_of lca /\
                     fst last1 <> fst last2 /\ 
-                    concrete_merge_pre (v_of lca) (do (v_of s1) last1) (do (v_of s2) last2) /\
-                    last (resolve_conflict last1 last2) <> last1 /\
-                    concrete_merge_pre (v_of lca) (do (v_of s1) last1) (v_of s2) /\
-                      
-                    (forall id id1. mem_id id (ops_of lca) /\ mem_id id1 (diff (ops_of s1) (ops_of lca)) ==> lt id id1) /\
-                    (forall id id1. mem_id id (ops_of lca) /\ mem_id id1 (diff (ops_of s2) (ops_of lca)) ==> lt id id1) /\
-                    (forall id. mem_id id (diff (ops_of s1) (ops_of lca)) ==> not (mem_id id (diff (ops_of s2) (ops_of lca)))))
+                    (exists l2. (do (v_of s2) last2 == apply_log (v_of lca) l2)) /\
+                    (exists l1. (do (v_of s1) last1 == apply_log (v_of lca) l1)) /\
+                    last (resolve_conflict last1 last2) <> last1)
          
           (ensures (eq (do (concrete_merge (v_of lca) (do (v_of s1) last1) (v_of s2)) last2)
-                         (concrete_merge (v_of lca) (do (v_of s1) last1) (do (v_of s2) last2)))) = 
-  assert (fst last1 < fst last2);
-  assert (do (concrete_merge (v_of lca) (do (v_of s1) last1) (v_of s2)) last2 =
-         (cons (fst last2) (cons (fst last1) (v_of lca))));
-  assert ((do (v_of s1) last1) = cons (fst last1) (v_of lca));
-  let s = fst (split (cons (fst last1) (v_of lca)) (length (cons (fst last1) (v_of lca)) - length (v_of lca))) in
-  lemma_split (cons (fst last1) (v_of lca)) (length (cons (fst last1) (v_of lca)) - length (v_of lca));
-  lemma_mem_append s (v_of lca);
-  assert (diff_s (cons (fst last1) (v_of lca)) (v_of lca) == cons (fst last1) empty);
-  assert ((do (v_of s2) last2) = cons (fst last2) (v_of lca));
-  let s = fst (split (cons (fst last2) (v_of lca)) (length (cons (fst last2) (v_of lca)) - length (v_of lca))) in
-  lemma_split (cons (fst last2) (v_of lca)) (length (cons (fst last2) (v_of lca)) - length (v_of lca));
-  lemma_mem_append s (v_of lca);
-  assert (diff_s (cons (fst last2) (v_of lca)) (v_of lca) == cons (fst last2) empty); 
+                       (concrete_merge (v_of lca) (do (v_of s1) last1) (do (v_of s2) last2)))) =
+  assert (do (concrete_merge (v_of lca) (do (v_of s1) last1) (v_of s2)) last2 ==
+          cons (fst last2) (cons (fst last1) (v_of lca)));
+  lemma_mem_append (create 1 (fst last1)) (v_of lca);
+  append_assoc (create 1 (fst last2)) (create 1 (fst last1)) (v_of lca);
+  assert (cons (fst last2) (cons (fst last1) (v_of lca)) ==
+          Seq.append (cons (fst last2) (cons (fst last1) empty)) (v_of lca));
+  ()
   
-  union_single (cons (fst last2) empty) (cons (fst last1) empty) (fst last2) (fst last1);
-  let u = union_s (cons (fst last2) empty) (cons (fst last1) empty) in
-  lem_app (fst last2) (fst last1) (v_of lca);
-  assert (Seq.append u (v_of lca) == (cons (fst last2) (cons (fst last1) (v_of lca)))); 
-  assert (concrete_merge (v_of lca) (do (v_of s1) last1) (do (v_of s2) last2) ==
-          (cons (fst last2) (cons (fst last1) (v_of lca)))); ()
-          
 let linearizable_gt0_base (lca s1 s2:st) (last1 last2:op_t)
-  : Lemma (requires is_prefix (ops_of lca) (ops_of s1) /\
-                    is_prefix (ops_of lca) (ops_of s2) /\
-                    ops_of s1 == ops_of lca /\ ops_of s2 == ops_of lca /\
+  : Lemma (requires consistent_branches lca s1 s2 /\
+                    ops_of s1 = ops_of lca /\ ops_of s2 = ops_of lca /\
                     fst last1 <> fst last2 /\ 
-                    concrete_merge_pre (v_of lca) (do (v_of s1) last1) (do (v_of s2) last2) /\
-                    (last (resolve_conflict last1 last2) = last1 ==>
-                      concrete_merge_pre (v_of lca) (v_of s1) (do (v_of s2) last2)) /\
-                
-                    (last (resolve_conflict last1 last2) <> last1 ==>
-                      concrete_merge_pre (v_of lca) (do (v_of s1) last1) (v_of s2)) /\
-                      
-                    (forall id id1. mem_id id (ops_of lca) /\ mem_id id1 (diff (ops_of s1) (ops_of lca)) ==> lt id id1) /\
-                    (forall id id1. mem_id id (ops_of lca) /\ mem_id id1 (diff (ops_of s2) (ops_of lca)) ==> lt id id1) /\
-                    (forall id. mem_id id (diff (ops_of s1) (ops_of lca)) ==> not (mem_id id (diff (ops_of s2) (ops_of lca)))))
+                    (exists l2. (do (v_of s2) last2 == apply_log (v_of lca) l2)) /\
+                    (exists l1. (do (v_of s1) last1 == apply_log (v_of lca) l1)))
          
           (ensures (last (resolve_conflict last1 last2) = last1 ==>
                       (eq (do (concrete_merge (v_of lca) (v_of s1) (do (v_of s2) last2)) last1)
@@ -463,109 +249,63 @@ let linearizable_gt0_base (lca s1 s2:st) (last1 last2:op_t)
 
                    (last (resolve_conflict last1 last2) <> last1 ==>
                       (eq (do (concrete_merge (v_of lca) (do (v_of s1) last1) (v_of s2)) last2)
-                         (concrete_merge (v_of lca) (do (v_of s1) last1) (do (v_of s2) last2))))) = 
-  if last (resolve_conflict last1 last2) = last1
-    then linearizable_gt0_base_last1 lca s1 s2 last1 last2
+                         (concrete_merge (v_of lca) (do (v_of s1) last1) (do (v_of s2) last2))))) =
+  if last (resolve_conflict last1 last2) = last1 then
+    linearizable_gt0_base_last1 lca s1 s2 last1 last2
   else linearizable_gt0_base_last2 lca s1 s2 last1 last2
 
 let linearizable_gt0_ind (lca s1 s2:st) (last1 last2:op_t)
-  : Lemma (requires is_prefix (ops_of lca) (ops_of s1) /\
-                    is_prefix (ops_of lca) (ops_of s2) /\
-                    length (ops_of s2) > length (ops_of lca) /\
+  : Lemma (requires consistent_branches_s2_gt0 lca s1 s2 /\
                     fst last1 <> fst last2 /\
-                    concrete_merge_pre (v_of lca) (do (v_of s1) last1) (do (v_of s2) last2) /\
-                    (forall id id1. mem_id id (ops_of lca) /\ mem_id id1 (diff (ops_of s1) (ops_of lca)) ==> lt id id1) /\
-                    (forall id id1. mem_id id (ops_of lca) /\ mem_id id1 (diff (ops_of s2) (ops_of lca)) ==> lt id id1) /\
-                    (forall id. mem_id id (diff (ops_of s1) (ops_of lca)) ==> not (mem_id id (diff (ops_of s2) (ops_of lca)))) /\
-          
+                    (exists l1. (do (v_of s1) last1 == apply_log (v_of lca) l1)) /\
+                    (exists l2. (do (v_of s2) last2 == apply_log (v_of lca) l2)) /\
                     (let s2' = inverse_st s2 in
-                    (last (resolve_conflict last1 last2) = last1 ==>
-                      concrete_merge_pre (v_of lca) (v_of s1) (do (v_of s2') last2) /\
-                      concrete_merge_pre (v_of lca) (do (v_of s1) last1) (do (v_of s2') last2) /\
-                      concrete_merge_pre (v_of lca) (v_of s1) (do (v_of s2) last2)) /\
-                   
-                    (last (resolve_conflict last1 last2) <> last1 ==>
-                      concrete_merge_pre (v_of lca) (do (v_of s1) last1) (v_of s2') /\
-                      concrete_merge_pre (v_of lca) (do (v_of s1) last1) (do (v_of s2') last2) /\
-                      concrete_merge_pre (v_of lca) (do (v_of s1) last1) (v_of s2)) /\
-                      
-                     is_prefix (ops_of lca) (ops_of s2') /\
-                     (forall id id1. mem_id id (ops_of lca) /\ mem_id id1 (diff (ops_of s2') (ops_of lca)) ==> lt id id1) /\
-                     (forall id. mem_id id (diff (ops_of s1) (ops_of lca)) ==> not (mem_id id (diff (ops_of s2') (ops_of lca))))))
+                    (exists l2. (do (v_of s2') last2 == apply_log (v_of lca) l2)) /\
+                    (exists l2. (v_of s2' == apply_log (v_of lca) l2)) /\
+                    (exists l1. (v_of s1 == apply_log (v_of lca) l1)) /\
+                    (exists l2. (v_of s2 == apply_log (v_of lca) l2)) /\
+                    consistent_branches lca s1 s2'))
        
           (ensures (let s2' = inverse_st s2 in
-                   (last (resolve_conflict last1 last2) = last1 /\
+                   ((last (resolve_conflict last1 last2) = last1 /\
                     eq (do (concrete_merge (v_of lca) (v_of s1) (do (v_of s2') last2)) last1)
-                       (concrete_merge (v_of lca) (do (v_of s1) last1) (do (v_of s2') last2)) ==>
+                       (concrete_merge (v_of lca) (do (v_of s1) last1) (do (v_of s2') last2))) ==>
                     (eq (do (concrete_merge (v_of lca) (v_of s1) (do (v_of s2) last2)) last1)
                         (concrete_merge (v_of lca) (do (v_of s1) last1) (do (v_of s2) last2)))) /\
                           
-                   (ops_of s1 = ops_of lca /\
+                   ((ops_of s1 = ops_of lca /\
                     last (resolve_conflict last1 last2) <> last1 /\
                     eq (do (concrete_merge (v_of lca) (do (v_of s1) last1) (v_of s2')) last2)
-                       (concrete_merge (v_of lca) (do (v_of s1) last1) (do (v_of s2') last2)) ==>
+                       (concrete_merge (v_of lca) (do (v_of s1) last1) (do (v_of s2') last2))) ==>
                     (eq (do (concrete_merge (v_of lca) (do (v_of s1) last1) (v_of s2)) last2)
-                        (concrete_merge (v_of lca) (do (v_of s1) last1) (do (v_of s2) last2)))))) = admit ()
+                        (concrete_merge (v_of lca) (do (v_of s1) last1) (do (v_of s2) last2)))))) = admit()
 
 let linearizable_gt0_ind1 (lca s1 s2:st) (last1 last2:op_t)
-  : Lemma (requires is_prefix (ops_of lca) (ops_of s1) /\
-                    is_prefix (ops_of lca) (ops_of s2) /\
-                    Seq.length (ops_of s1) > Seq.length (ops_of lca) /\
+  : Lemma (requires consistent_branches_s1_gt0 lca s1 s2 /\
                     fst last1 <> fst last2 /\
-                    concrete_merge_pre (v_of lca) (do (v_of s1) last1) (do (v_of s2) last2) /\
-                    (forall id id1. mem_id id (ops_of lca) /\ mem_id id1 (diff (ops_of s1) (ops_of lca)) ==> lt id id1) /\
-                    (forall id id1. mem_id id (ops_of lca) /\ mem_id id1 (diff (ops_of s2) (ops_of lca)) ==> lt id id1) /\
-                    (forall id. mem_id id (diff (ops_of s1) (ops_of lca)) ==> not (mem_id id (diff (ops_of s2) (ops_of lca)))) /\
-
+                    (exists l1. (do (v_of s1) last1 == apply_log (v_of lca) l1)) /\
+                    (exists l2. (do (v_of s2) last2 == apply_log (v_of lca) l2)) /\
                     (let s1' = inverse_st s1 in
-                    (last (resolve_conflict last1 last2) = last1 ==>
-                      concrete_merge_pre (v_of lca) (v_of s1) (do (v_of s2) last2) /\
-                      concrete_merge_pre (v_of lca) (v_of s1') (do (v_of s2) last2) /\
-                      concrete_merge_pre (v_of lca) (do (v_of s1') last1) (do (v_of s2) last2)) /\
-                   
-                    (last (resolve_conflict last1 last2) <> last1 ==>
-                      concrete_merge_pre (v_of lca) (do (v_of s1) last1) (v_of s2) /\
-                      concrete_merge_pre (v_of lca) (do (v_of s1') last1) (v_of s2) /\
-                      concrete_merge_pre (v_of lca) (do (v_of s1') last1) (do (v_of s2) last2)) /\
-                   
-                    is_prefix (ops_of lca) (ops_of s1') /\
-                    (forall id id1. mem_id id (ops_of lca) /\ mem_id id1 (diff (ops_of s1') (ops_of lca)) ==> lt id id1) /\
-                    (forall id. mem_id id (diff (ops_of s1') (ops_of lca)) ==> not (mem_id id (diff (ops_of s2) (ops_of lca))))))
+                    (exists l1. (do (v_of s1') last1 == apply_log (v_of lca) l1)) /\
+                    (exists l1. (v_of s1' == apply_log (v_of lca) l1)) /\
+                    (exists l1. (v_of s1 == apply_log (v_of lca) l1)) /\
+                    (exists l2. (v_of s2 == apply_log (v_of lca) l2)) /\
+                    consistent_branches lca s1' s2))
         
           (ensures (let s1' = inverse_st s1 in
-                   (ops_of s2 = ops_of lca /\
+                   ((ops_of s2 = ops_of lca /\
                    last (resolve_conflict last1 last2) = last1 /\
                    eq (do (concrete_merge (v_of lca) (v_of s1') (do (v_of s2) last2)) last1)
-                      (concrete_merge (v_of lca) (do (v_of s1') last1) (do (v_of s2) last2)) ==>
+                      (concrete_merge (v_of lca) (do (v_of s1') last1) (do (v_of s2) last2))) ==>
                    eq (do (concrete_merge (v_of lca) (v_of s1) (do (v_of s2) last2)) last1)
                       (concrete_merge (v_of lca) (do (v_of s1) last1) (do (v_of s2) last2))) /\
 
-                   (last (resolve_conflict last1 last2) <> last1 /\
+                   ((last (resolve_conflict last1 last2) <> last1 /\
                     eq (do (concrete_merge (v_of lca) (do (v_of s1') last1) (v_of s2)) last2)
                        (concrete_merge (v_of lca) (do (v_of s1') last1) (do (v_of s2) last2)) ==>
                     eq (do (concrete_merge (v_of lca) (do (v_of s1) last1) (v_of s2)) last2)
-                       (concrete_merge (v_of lca) (do (v_of s1) last1) (do (v_of s2) last2))))) = admit ()
-                       
-let linearizable_gt0_merge_pre (lca s1 s2:st) (last1 last2:op_t)
-  : Lemma (requires is_prefix (ops_of lca) (ops_of s1) /\
-                    is_prefix (ops_of lca) (ops_of s2) /\
-                    Seq.length (ops_of s1) > Seq.length (ops_of lca) /\
-                    Seq.length (ops_of s2) > Seq.length (ops_of lca) /\
-                    (forall id id1. mem_id id (ops_of lca) /\ mem_id id1 (diff (ops_of s1) (ops_of lca)) ==> lt id id1) /\
-                    (forall id id1. mem_id id (ops_of lca) /\ mem_id id1 (diff (ops_of s2) (ops_of lca)) ==> lt id id1) /\
-                    (forall id. mem_id id (diff (ops_of s1) (ops_of lca)) ==> not (mem_id id (diff (ops_of s2) (ops_of lca)))) /\
-                    last1 == last (ops_of s1) /\
-                    last2 == last (ops_of s2) /\             
-                    fst last1 <> fst last2 /\
-                    concrete_merge_pre (v_of lca) (v_of s1) (v_of s2))
-       
-          (ensures (last (resolve_conflict last1 last2) = last1 ==>
-                       concrete_merge_pre (v_of lca) (v_of (inverse_st s1)) (v_of s2)) /\
+                       (concrete_merge (v_of lca) (do (v_of s1) last1) (do (v_of s2) last2)))))) = admit()
 
-                   (last (resolve_conflict last1 last2) <> last1 ==>
-                       concrete_merge_pre (v_of lca) (v_of s1) (v_of (inverse_st s2)))) = admit()
-  
-                       
 ////////////////////////////////////////////////////////////////
 //// Sequential implementation //////
 
